src/Init/Data/List/Perm.lean
@@ -470,8 +470,10 @@ theorem Perm.flatten {l₁ l₂ : List (List α)} (h : l₁ ~ l₂) : l₁.flatt
 
 @[deprecated Perm.flatten (since := "2024-10-14")] abbrev Perm.join := @Perm.flatten
 
-theorem Perm.bind_right {l₁ l₂ : List α} (f : α → List β) (p : l₁ ~ l₂) : l₁.bind f ~ l₂.bind f :=
+theorem Perm.flatMap_right {l₁ l₂ : List α} (f : α → List β) (p : l₁ ~ l₂) : l₁.flatMap f ~ l₂.flatMap f :=
   (p.map _).flatten
+
+@[deprecated Perm.flatMap_right (since := "2024-10-16")] abbrev Perm.bind_right := @Perm.flatMap_right
 
 theorem Perm.eraseP (f : α → Bool) {l₁ l₂ : List α}
     (H : Pairwise (fun a b => f a → f b → False) l₁) (p : l₁ ~ l₂) : eraseP f l₁ ~ eraseP f l₂ := by
